store/game.v
@@ -36,8 +36,8 @@ Definition game : val := λ: <>,
   let: "c" := init_network #() in
 
   (* Create key pairs and give verification keys to attacker *)
-  let: "skI" := mksigkey #() in
-  let: "skR" := mksigkey #() in
+  let: "skI" := mk_sign_key #() in
+  let: "skR" := mk_sign_key #() in
   let: "vkI" := vkey "skI" in
   let: "vkR" := vkey "skR" in
   send "c" "vkI";; send "c" "vkR";;
@@ -102,9 +102,9 @@ iMod (iso_dh_ctx_alloc with "enc_tok") as "[#? enc_tok]" => //.
 iMod (RPC.ctx_alloc with "[$] [//]") as "[#? enc_tok]"; first solve_ndisj.
 iMod (store_ctx_alloc with "[$] [//]") as "[#? _]" => //; first solve_ndisj.
 wp_apply wp_init_network => //. iIntros "%c #cP". wp_pures.
-wp_apply (wp_mksigkey with "[]"); eauto.
+wp_apply (wp_mk_sign_key with "[]"); eauto.
 iIntros "%skI #p_vkI #sign_skI s_skI tokenI". wp_pures.
-wp_pures. wp_apply (wp_mksigkey with "[]"); eauto.
+wp_pures. wp_apply (wp_mk_sign_key with "[]"); eauto.
 iIntros "%skR #p_vkR #sign_skR s_skR tokenR". wp_pures.
 wp_apply wp_vkey. wp_pures.
 wp_apply wp_vkey. wp_pures.
